nola/iris/store_deriv.v
@@ -186,3 +186,70 @@ Section store_deriv.
     iApply ("PQR" with "[//] [//] [//] Px Qx").
   Qed.
 End store_deriv.
+
+(** ** Constructor *)
+
+From nola.iris Require Import cif.
+
+(** [storeCT]: Constructor for [store] *)
+Variant storeCT_id := .
+Definition storeCT :=
+  Cifcon storeCT_id bool (λ _, Empty_set) (λ _, unit) (λ _, unitO) _.
+(** [storeC]: [storeCT] registered *)
+Notation storeC := (inC storeCT).
+
+Section storeC.
+  Context `{!storeC CON} {Σ}.
+  Implicit Type Px : cif CON Σ.
+  (** Formulas *)
+  Definition cif_store Px : cif CON Σ :=
+    cif_ecustom storeCT true nullary (unary Px) ().
+  Definition cif_pstore Px : cif CON Σ :=
+    cif_ecustom storeCT false nullary (unary Px) ().
+  (** The formulas are non-expansive *)
+  #[export] Instance cif_store_ne : NonExpansive cif_store.
+  Proof. move=> ????. apply cif_ecustom_ne; solve_proper. Qed.
+  #[export] Instance cif_store_proper : Proper ((≡) ==> (≡)) cif_store.
+  Proof. apply ne_proper, _. Qed.
+  #[export] Instance cif_pstore_ne : NonExpansive cif_pstore.
+  Proof. move=> ????. apply cif_ecustom_ne; solve_proper. Qed.
+  #[export] Instance cif_pstore_proper : Proper ((≡) ==> (≡)) cif_pstore.
+  Proof. apply ne_proper, _. Qed.
+  (** The formulas are productive *)
+  #[export] Instance cif_store_productive : Productive cif_store.
+  Proof.
+    move=> ????. apply cif_ecustom_preserv_productive=>//.
+    by apply fun_proeq_later.
+  Qed.
+  #[export] Instance cif_pstore_productive : Productive cif_pstore.
+  Proof.
+    move=> ????. apply cif_ecustom_preserv_productive=>//.
+    by apply fun_proeq_later.
+  Qed.
+
+  Context `{!storeGS (cifOF CON) Σ, !storeJ (cifO CON Σ) JUDG}.
+  (** Semantics of [storeCT] *)
+  Definition storeCT_sem δ b : cif CON Σ → iProp Σ :=
+    if b then store δ else pstore δ.
+  #[export] Program Instance storeCT_ecsem : Ecsem storeCT CON JUDG Σ :=
+    ECSEM (λ _ δ b _ Φx _, storeCT_sem δ b (Φx ())) _.
+  Next Obligation.
+    move=>/= ??*? b ?*?? eqv ?*. case b=>/=; f_equiv; apply eqv.
+  Qed.
+End storeC.
+(** [storeC] semantics registered *)
+Notation storeCS := (inCS storeCT).
+
+(** Reify into formulas *)
+Section storeC.
+  Context `{!Csem CON JUDG Σ, !Jsem JUDG (iProp Σ), !storeGS (cifOF CON) Σ,
+    !storeC CON, !storeJ (cifO CON Σ) JUDG, !storeCS CON JUDG Σ,
+    !storeJS (cifOF CON) JUDG Σ}.
+
+  #[export] Program Instance store_as_cif {Px} :
+    AsCif CON (λ δ, store δ Px) := AS_CIF (cif_store Px) _.
+  Next Obligation. move=>/= *. by rewrite sem_ecustom. Qed.
+  #[export] Program Instance pstore_as_cif {Px} :
+    AsCif CON (λ δ, pstore δ Px) := AS_CIF (cif_pstore Px) _.
+  Next Obligation. move=>/= *. by rewrite sem_ecustom. Qed.
+End storeC.
